---  
layout: mathjax  
---  
  
# 47. Производная суммы и произведения двух функций.  
  
### $f, g~-~$дифференцируемы в $x_0$. Тогда:  
$(f+g)'=f'+g'\newline  
(fg)'=f'g+fg'$  
Доказательство:  
$(f+g)'=\lim\limits_{x\to x_0}\dfrac{f(x)+g(x)-f(x_0)-g(x_0)}{x-x_0}=\newline=\lim\limits_{x\to x_0}\dfrac{f(x)-f(x_0)}{x-x_0}+\lim\limits_{x\to x_0}\dfrac{g(x)-g(x_0)}{x-x_0}=f'+g' ~~ \scriptsize \blacksquare$  
  
$(fg)'=\lim\limits_{x\to x_0}\dfrac{f(x)g(x)-f(x_0)g(x_0)}{x-x_0}=\newline=  
\lim\limits_{x\to x_0}\dfrac{f(x)g(x)-f(x_0)g(x)+f(x_0)g(x)-f(x_0)g(x_0)}{x-x_0}=\newline=\lim\limits_{x\to x_0}\dfrac{g(x)(f(x)-f(x_0))+f(x_0)(g(x)-g(x_0))}{x-x_0}=\newline=  
\lim\limits_{x\to x_0}\dfrac{g(x)(f(x)-f(x_0))}{x-x_0}+\lim\limits_{x\to x_0}\dfrac{f(x_0)(g(x)-g(x_0))}{x-x_0}=\newline=f'(x_0)g(x_0)+f(x_0)g'(x_0) ~~ \scriptsize \blacksquare$  
