---  
layout: mathjax  
---  
  
# 48. Производная разности и отношения двух функций.  
  
### $f, g~-~$дифференцируемы в $x_0$. Тогда:  
$(f-g)'=f'-g'\newline  
(\dfrac{f}{g})'=\dfrac{f'g-fg'}{g^2}$  
Доказательство:  
$(f-g)'=\lim\limits_{x\to x_0}\dfrac{f(x)-g(x)-f(x_0)+g(x_0)}{x-x_0}=\newline=\lim\limits_{x\to x_0}\dfrac{f(x)-f(x_0)}{x-x_0}-\lim\limits_{x\to x_0}\dfrac{g(x)-g(x_0)}{x-x_0}=f'-g' ~~ \scriptsize \blacksquare$  
  
$(\dfrac{1}{g})'=\lim\limits_{x\to x_0}\dfrac{\frac{1}{g(x)}-\frac{1}{g(x_0)} }{x-x_0}=\lim\limits_{x\to x_0}\dfrac{\frac{g(x_0)-g(x)}{g(x)g(x_0)} }{x-x_0}=\newline=\lim\limits_{x\to x_0}\dfrac{g(x_0)-g(x)}{g(x)g(x_0)(x-x_0)}=\lim\limits_{x\to x_0}\dfrac{g(x_0)-g(x)}{x-x_0} \* \dfrac{1}{g(x)g(x_0)}=\\=-\dfrac{g'(x_0)}{g(x_0)^2}$  
$(\dfrac{f}{g})'=(f*\dfrac{1}{g})'=f'*\dfrac{1}{g}+f*(\dfrac{1}{g})'=\dfrac{f'}{g}-\dfrac{fg'}{g^2}=\newline=\dfrac{f'g-fg'}{g^2}  ~~ \scriptsize \blacksquare$  
